Challenge/Ripemd160/Submission/Proofs/Bytecode/Table80Setup.lean
@@ -359,7 +359,6 @@ def storesTemplate : List Instr :=
     .op .POP,
     .push ⟨1, by decide⟩ (UInt256.ofNat 25),
     .push ⟨1, by decide⟩ (UInt256.ofNat 24),
-    .push ⟨1, by decide⟩ (UInt256.ofNat 63),
     .push ⟨1, by decide⟩ (UInt256.ofNat 26),
     .push ⟨1, by decide⟩ (UInt256.ofNat 27),
     .push ⟨1, by decide⟩ (UInt256.ofNat 22) ]
@@ -420,7 +419,6 @@ def padTemplate : List Instr :=
     .op .MSTORE,
     .push ⟨1, by decide⟩ (UInt256.ofNat 25),
     .push ⟨1, by decide⟩ (UInt256.ofNat 24),
-    .push ⟨1, by decide⟩ (UInt256.ofNat 63),
     .push ⟨1, by decide⟩ (UInt256.ofNat 26),
     .push ⟨1, by decide⟩ (UInt256.ofNat 27),
     .push ⟨1, by decide⟩ (UInt256.ofNat 22) ]
